\graphicspath{{figures/series/}}
\chapter{Partial Derivatives}\label{chap par der}

\section{Partial Derivatives}
\begin{defn}
\[f(x) \quad x \in R \quad \text{\tssteelblue{single variable}}\] 
\[f(x, y) \quad x, y \in R \quad \text{\tssteelblue{multi variables}}\]
\end{defn}
\begin{eg}
\[z = f(x, y) = \sqrt{9 - x^2 - y^2}\]
\begin{itemize}
\item Domain
\[9 - x^2 - y^2 \geq 0\] 
\[x^2 +y^2 \leq 9\]
\(\implies\) Domain is \(\{(x, y) | x^2 + y^2 \leq 9\}\)
\item Range
\[0 \leq x^2 + y^2 \leq 9\] 
\[0 \leq 9 - x^2 - y^2 \leq 9\]
\[0 \leq \sqrt{9 - x^2 - y^2} \leq 3\]
\(\implies\) Range is \(0 \leq z \leq 3\)
\item Graph
\[z = \sqrt{9 - x^2 - y^2}\]
\[z^2 = 9 - x^2 - y^2\]
\[x^2 + y^2 + z^2 = 9\]
\[(x - 0)^2 + (y - 0)^2 + (z - 0)^2 = 3^2\]
\(\implies\) 上半球面(sphere) \quad center = \((0, 0)\) \quad radius = \(3\) 
\item Level Curve（等高線）
\[z = \sqrt{9 - x^2 - y^2}\]
\[k = 9 - x^2 - y^2\]
\[x^2 + y^2 = 9 - k\]
\[0 \leq k \leq 9\]
\[k = 0 \quad x^2 + y^2 = 3^2\]
\[k = 1 \quad x^2 + y^2 = (2 \sqrt{2})^2\]
\end{itemize}
\end{eg}
\section{Limit and Continuity}
\begin{itemize}
\item 1D \(\implies \displaystyle \lim_{x \to a} f(x)\)
\item 2D \(\implies \displaystyle \lim_{(x, y) \to (a, b)} f(x, y)\)
\end{itemize}
\begin{defn}
\(\displaystyle \lim_{A \to B} f(A) = L\) \ if \ \(\forall \epsilon > 0 \quad \exists \delta > 0\)\\
s.t. if \(d(A, B) < \delta\), then 
\[|f(A) - L| < \epsilon\]
\end{defn}
\begin{eg}
Does \(\displaystyle \lim_{(x, y) \to (0, 0)} \frac{x^2 - y^2}{x^2 + y^2}\) exists? \quad \tssteelblue{homogeneous 齊次}

\soln \ \\
Along the line \(y = mx \quad m\): const\\
\[\displaystyle \lim_{(x, m) \to (0, 0)} \frac{x^2 - y^2}{x^2 + y^2} = \displaystyle \lim_{x \to 0} \frac{\cancel{x^2} (1 - m^)}{\cancel{x^2} (1 + m^2)} = \displaystyle \frac{1 - m^2}{1 + m^2} \quad \tssteelblue{\text{depend on } m}\]
\(\implies\) The limit doesn't exist
\end{eg}
\begin{eg}
Does \(\displaystyle \lim_{(x, y) \to (0, 0)} \frac{xy^2}{x^2 + y^4}\) exists?

\soln
\[y = mx^k \quad k: \text{ const}\]
\[\displaystyle \frac{x \cdot m^2 x^{2k}}{x^2 + m^4x^{4k}} = \frac{m^2 x^{2k + 1}}{x^2 + mx^4k}\]
\[2k + 1 = 2 = 4k\]
\[k = \frac{1}{2}\]
Along \(y = mx^{\frac{1}{2}}\)
\[\displaystyle \lim_{(x, mx^{\frac{1}{2}}) \to (0, 0)} \frac{x \cdot m^2x}{x^2 + m^4x^2} = \lim_{x \to 0} \frac{\cancel{x^2} m^2}{\cancel{x^2}(1 + m^4)} = \frac{m^2}{1 + m^4} \quad \tssteelblue{\text{depend on }m}\]
\(\implies\) The limit doesn't exist
\end{eg}
\begin{eg}
Find \(\displaystyle \lim_{(x, y) \to (0, 0)} \frac{x^2y}{x^2 + y^2}\)

\soln 1
\[\displaystyle \Big| \frac{x^2y}{x^2 + y^2} \Big| = \Big| \frac{x^2}{x^2 + y^2} \Big| \Big|y\Big| \leq 1|y| = |y|\]
\[\displaystyle \lim_{(x, y) \to (0, 0)} 0 \leq \lim_{(x, y) \to (0, 0)} \Big| \frac{x^2y}{x^2 + y^2} \Big| \leq \lim_{(x, y) \to (0, 0)} |y|\]
By Squeeze Theorem
\[\displaystyle \lim_{(x, y) \to (0, 0)} \Big| \frac{x^2y}{x^2 + y^2} \Big| = 0 = \lim_{(x, y) \to (0, 0)} \frac{x^2y}{x^2 + y^2}\]
\soln 2\\
Use polar coordinates \((x, y) \to (r, \theta)\)
\[x = r\cos \theta \quad y = r\sin \theta\]
\[\displaystyle \lim_{(x, y) \to (0, 0)} \frac{x^2y}{x^2 + y^2} = \lim_{r \to 0} \frac{r^3 \cos^2 \theta \sin \theta}{r^2} = 0\]
\end{eg}
\begin{eg} 
Does \(\displaystyle \lim_{(x, y) \to (0, 0)} \frac{x^2 + \sin^2 y}{2x^2 + y^2}\) exists?

\soln Key: \(\displaystyle \lim_{y \to 0} \frac{\sin y}{y} = 1 \quad y = mx\)\\
Along \(y = mx\)
\[\begin{array}{rcl}
\displaystyle \lim_{(x, y) \to (0, 0)} \frac{x^2 + (\frac{\sin y}{mx})^2(mx)^2}{2x^2 + y^2} & = & \lim_{x \to 0} \frac{\cancel{x^2} +m^2\cancel{x^2}(\frac{\sin (mx)}{mx})^2}{2\cancel{x^2} + m^2\cancel{x^2}}\\
& = & \displaystyle \frac{1}{1 + m^2} \lim_{x \to 0} (1 + m^2 (\frac{\sin (mx)}{mx})^2)\\
& = & \displaystyle \frac{1}{1 + m^2}(1 + m^2 \cdot 1)
\end{array}\]
\(\implies\) The limit doesn't exist
\end{eg}
\begin{notn}
\begin{itemize}
\item \(f(x)\) is continue at \(a\) if \(\displaystyle \lim_{x \to a} f(x) = \underline{f(a)}\)
\item \(f(x, y)\) is continue at \((x_0, y_0)\) if \(\displaystyle \lim_{(x, y) \to (x_0, y_0)} f(x, y) = \underline{f(x_0, y_0)}\)
\end{itemize}
\end{notn}
\begin{eg} 
Find \(a\) such that \(f(x, y) = \left\{ \begin{array}{ccl}
\displaystyle \frac{x^2 + y^2}{\sqrt{x^2 + y^2 + 1} - 1} &, & (x, y) \neq (0, 0)\\
a &, & (x, y) = (0, 0)
\end{array}\right.\) is conti. at \((0, 0)\)

\soln 1\\
We need \(\displaystyle \lim_{(x, y) \to (0, 0)}f(x, y) = f(0, 0)\)
\[\begin{array}{rcl}
\text{LHS} & = & \displaystyle \lim_{(x, y) \to (0, 0)} \frac{x^2 + y^2}{\sqrt{x^2 + y^2 + 1} - 1} \cdot \frac{\sqrt{x^2 + y^2 + 1} + 1}{\sqrt{x^2 + y^2 + 1} + 1}\\
& = & \lim_{(x, y) \to (0, 0)} \frac{\cancel{(x^2 + y^2)} (\sqrt{x^2 + y^2 + 1} + 1)}{\cancel{x^2 + y^2}}\\
& = & 2 = a = \text{RHS}
\end{array}\]
\(\implies a = 2\)

\soln 2\\
Use \(x = r \cos \theta \quad y = r \sin \theta\)
\[\begin{array}{rcl}
\text{LHS} & = & \displaystyle \lim_{r \to 0} \frac{r^2}{\sqrt{r^2 + 1} - 1}\\
& \vdots &\\
& = & 2
\end{array}\]
\end{eg}
\section{First Partial Derivatives}
Recall: \(\displaystyle f'(a) = \lim_{h \to 0} \frac{f(a + h) - f(a)}{h}\)
\begin{itemize}
\item \(\displaystyle \frac{\partial}{\partial x} (x, y)\Big|_{(a, b)} = \lim_{h \to 0} \frac{f(a + h, b) - f(a, b)}{h}\)
\item \( \displaystyle \frac{\partial}{\partial y} f(x, y) \Big|_{(a, b)} = \lim_{h \to 0} \frac{f(a, b+h) - f(a, b)}{h}\)
\end{itemize}
\begin{notn}
\[\displaystyle \frac{\partial}{\partial x} f(x, y) = \frac{\partial f(x, y)}{\partial x} = f_x (x, y) = \partial x f(x, y)\]
\end{notn}
\begin{eg}
\(f(x, y) = x^2 + xy + 2y^2\). Find \(f_x\) and \(f_y\)

\soln
\[\begin{array}{rcl}
f_x & = & \displaystyle \frac{\partial}{\partial x} f(x, y)\\
& = & \displaystyle \frac{\partial}{\partial x} (x^2 + xy + 2y^2)\\
& = & 2x + y + 0
\end{array}\]
\[\begin{array}{rcl}
f_y & = & \displaystyle \frac{\partial}{\partial y} f(x, y)\\
& = & \displaystyle \frac{\partial}{\partial y} (x^2 + xy +2y^2)\\
& = & 0 + x + 4y
\end{array}\]
\end{eg}
\section{Second Partial Derivatives}
\begin{itemize}
\item \((f_x)_x = f_{xx} = \displaystyle \frac{\partial}{\partial x} (\frac{\partial f(x, y)}{\partial x}) = \frac{\partial^2 f(x, y)}{\partial x^2}\)
\item \((f_x)_y = f_{xy} = \displaystyle \frac{\partial}{\partial y} (\frac{\partial f(x, y)}{\partial x}) = \frac{\partial^2 f(x, y)}{\partial y \partial x}\)
\item \((f_y)_x = f_{yx} = \displaystyle \frac{\partial}{\partial x} (\frac{\partial f(x, y)}{\partial y}) = \frac{\partial^2 f(x, y)}{\partial x \partial y}\)
\item \((f_y)_y = f_{yy} = \displaystyle \frac{\partial}{\partial y} (\frac{\partial f(x, y)}{\partial y}) = \frac{\partial^2 f(x, y)}{\partial y^2}\)
\end{itemize}
\begin{eg}
\[f(x, y) = x^2 + xy + 2y^2\]

\[\begin{array}{rcl}
f_{xx} = (f_x)_x = 2 & \quad \quad & f_{yx} = (f_y)_x = 1\\
f_{xy} = (f_x)_y = 1 & \quad \quad & f_{yy} = (f_y)_y = 4
\end{array}\]
\end{eg}
\begin{eg}
\(u(x, y) = e^x \sin y\). Find \(u_{xx} + u_{yy}\).

\soln
\[u = e^x \sin y\]
\[u_x = e^x \sin y\]
\[u_{xx} = (u_x)_x = e^x \sin y\]
\[u_y = e^x \cos y\]
\[u_{yy} = (u_y)_y = e^x (- \sin y)\]
\(\implies u_{xx} + u_{yy} = 0\) \quad \tssteelblue{Laplace Equation}
\end{eg}
\begin{theorem}[Clairaut Theorem]
If \(f_{xy}\) and \(f_{yx}\) are conti in \(D\), then
\[f_{xy} = f_{yx} \text{ in } D\]
\end{theorem}
\begin{eg}
If you are told \(\exists\) a fcn. s.t. \(\left\{\begin{array}{rcl}
f_x & = & 2x + 3y\\
f_y & = & 4x - y
\end{array}\right.\). Believe it or not?

\soln
\[(f(x, y) \in c^2 \quad \text{兩次微分後連續}\]
\[\left\{\begin{array}{rclcrl}
f_x & = & 2x + 3y &\implies & f_{xy} = (f_x)_y = 3\\
f_y & = & 4x - y & \implies & f_{yx} = (f_y)_x = 4
\end{array}\right.\]
\(\implies\) I don't believe it.
\end{eg}
\begin{eg}
If \(u(x, t) = u(x - ct) \quad c:\text{ const}\). Find \(u_{tt} - c^2u_{xx}\)

\soln \ \\
Let \(z = x - ct\)
\[u_x = u_z \cdot z_x = u_z \cdot 1 = u_z\]
\[u_{xx} = (u_z)_z \cdot  z_x = u_{zz} \cdot 1 = u_{zz}\]
\[u_t = u_z \cdot z_t = u_z \cdot (-c) = -cu_z\]
\[u_{tt} = (-cu_z)_z) \cdot z_t = -c u_{zz}(-c) = c^2 {u_zz}\]
\[u_{tt} - c^2u_{xx} = c^2 u_{zz} - c^2u_{zz} = 0\]
\end{eg}
\begin{notn}
\begin{itemize}
\item Laplace Equation\\
\(u(x, y) = e^x \sin y \) satisfies \(u_{xx} + u{yy} = 0\)
\item Wave Equation\\
\(u(x, t) = u(x - ct)\) solves \(u_{tt} - c^2u_{xx} = 0\)
\end{itemize}
\end{notn}
\begin{eg}
\[u(x, t) = \sin (x - ct) \overset{c = 1}{=} \sin (x - t)\]
\[\begin{array}{rcl}
t = 0 &, & \sin x\\
t = 1 &, & \sin (x - 1)\\
t = 2 &, & \sin (x - 2)
\end{array}\]
\end{eg}
\section{Partial Derivatives by Implicit Differentiation}
\begin{eg}
If \(xyz = \cos (x + y + y)\). Find \(\displaystyle \frac{\partial z}{\partial x}( = z_x), \frac{\partial z}{\partial y} (= z_y)\)

\soln
\[z = z(x, y)\]
\[xyz(x, y) = \cos (x + y + z(x, y)) \quad \tssteelblue{\text{Product Rule}}\]
\[y(z + xz_x) = - \sin (x + y + z(x, y)) \cdot (1 + 0 + z_x) \quad \tssteelblue{\text{Chain Rule}}\]
\[yz + xyz_x = - \sin (x + y + z') - z_x \sin (x + y + z)\]
\[\displaystyle z_x = \frac{-yz - \sin (x + y + z)}{xy + \sin (x + y + z)}\]
\[\displaystyle z_y = \frac{-xz - \sin (x + y + z)}{xy + \sin (x + y +z)}\]
\end{eg}
\begin{eg}
\(\displaystyle f(x, y) = (\frac{1}{3} (x^3 + y^3))(e^{- \sin y})\). Find \(\displaystyle f_x (1, 0) = \frac{\partial f}{\partial x} \Big|_{(1, 0)}\)

\soln 1
\[f_x(x, y) = e^{\sin y} \cdot x^2\]
\[f_x(1, 0) = e^{- 0} \cdot 1^2 = 1\]

\soln 2
\[f(x, 0) = \frac{1}{3} x^3\]
\[f_x(x, o) = x^2\]
\[f_x(1, 0) = 1^2 = 1\]
\end{eg}
\begin{eg}
\[f(x, y) = \left\{\begin{array}{ccl}
\displaystyle \frac{x^3y - xy^3}{x^2 + y^2} &, & (x, y ) \neq (0, 0)\\
0 &, & (x, y) = (0, 0)
\end{array}\right.\]
\begin{itemize}
\item[(1)] Find \(f_x\) and \(f_y\) when \((x, y) \neq (0, 0)\)

\soln
\[\begin{array}{rcl}
f_x & = & \displaystyle \frac{(x^2 + y^2)(3x^2y - y^3) - (x^3y - xy^3)(2x)}{(x^2 + y^2)^2} \quad \tssteelblue{\text{Quotient Rule}}\\
& = & \displaystyle \frac{x^4 + 4x^2y^2 - y^4}{(x^2 + y^2)^2}\\
f_y & = & \displaystyle \frac{(x^2 + y^2)(x^3 - 3xy^2) - (x^3y - xy^3)(2y)}{(x^2 + y^2)^2}\\
& = & \displaystyle \frac{x(x^4 - 4x^2y^2 - y^4)}{(x^2 + y^2)^2}
\end{array}\]
\item[(2)] Find \(f_x(0, 0)\) and \(f_y(0, 0)\)

\soln
\[\begin{array}{rcl}
f_x(0, 0) & := & \displaystyle \lim_{h \to 0} \frac{f(0 + h, 0) - f(0, 0)}{h}\\
& = & \displaystyle \lim_{h \to 0} \frac{0 - 0}{h}\\
& = & 0\\
f_y(0, 0) & := & \displaystyle \lim_{h \to 0} \frac{f(0, h) - f(0, 0)}{h}\\
& = & 0
\end{array}\]
\item[(3)] Find \(f_{xy}(0, 0)\) and \(f_{yx}(0, 0)\)

\soln
\[\begin{array}{rcl}
(f_x)_y (0, 0) & = & g_y(0, 0)\\
& = & \displaystyle \lim_{h \to 0} \frac{g(o, h) - g(0, 0)}{h}\\
& = & \displaystyle \lim_{h \to 0} \frac{f_x(0, h) - f_x(0, 0)}{h}\\
& = & \displaystyle \lim_{h \to 0} \frac{\frac{h(-\cancel{h^4})}{\cancel{h^4}} - f_x(0, 0)}{h}\\
& = & \displaystyle \lim_{h \to 0} \frac{-\cancel{h}}{\cancel{h}}\\
& = & -1\\
(f_y)_x (0, 0) & = & J_x(0, 0)\\
& = & \displaystyle \lim_{h \to 0} \frac{J(h, o) - J(0, 0)}{h}\\
& = & \displaystyle \lim_{h \to 0} \frac{f_y(h, o) - f_y(0 , 0)}{h}\\
& = & \displaystyle \lim_{h \to 0} \frac{\frac{h^{\cancel5}}{\cancel{h^4}} - f_y(0, 0)}{h}\\
& = & \displaystyle \lim_{h \to 0} \frac{h}{h}\\
& = & 1
\end{array}\]
\end{itemize}
\end{eg}
\section{Tangent Planes}
\begin{notn}
\[z = f(x, y) \quad p = (x_0, y_0, z_0)\]
Q: Find the tangent plane of \(z = f(x, y)\) at \(P\)\\\\\\
\(c_1: z = f(x_0, y)\\
T_1\): tangent line of \(c_1\) at \(x_0\)\\
\(c_2: z = f(x, y_0)\\
T_x\): tangent line of \(c_2\) at \(y_0\)\\
\[a(x - x_0) + b(y - y_0) + c(z - z_0) = 0\]
If \(c \neq 0\)
\[\displaystyle \frac{a}{c} (x - x_0) + \frac{b}{c} (y - y_0) + (z - z_0) = 0\]
Normal Vector = \((A, B, 1)\)\\
\[A(x - x_0) + B(y - y_0) + (z - z_0) = 0\]
\begin{itemize}
\item \(x = x_0\)\\
\(T_1: B(y - y_0) + (z - z_0) = 0\\
\implies \displaystyle B = - \frac{z - z_0}{y - y_0} = - f_y(x_0, y_0)\)
\item \(y = y_0\)\\
\(T_2: A(x - x_0) + (z - z_0) = 0\\
\implies \displaystyle A = - \frac{z - z_0}{x - x_0} = - f_x(x_0, y_0)\)
\end{itemize}
\[(A, B, 1) = ( -f_x(x_0, y_0), -f_y(x_0, y_0), 1)\]
Tangent plane\\
\[z - f_x(x, y) = 0\]
\[\displaystyle (-f_x, -f_y, 1)|_{(x_0, y_0)}\]
\[F = z - f(x, y)\]
\[\displaystyle (F_x, F_y, F_z)|_{(x_0, y_0)}\]
\end{notn}
\begin{eg}
\(z = f(x, y) = 2x^2 + y^2\). Find the tangent plane of \(z = f(x, y)\) at \((1, 1, 3)\)

\soln \ \\
Normal vector is \((- f_x, -f_y, 1)|_{(1, 1)} = (-4x, -2y, 1)|_{(1, 1)} = (-4, -2, 1)\)\\
Tangent plane
\[-4(x - 1) - 2(y - 1) + (z - 3) = 0\]
\[-4x - 2y + z + 3 = 0\]
\end{eg}
\section{Linear Approximation}
\begin{notn}
\[z = f(x, y) \quad (x_0, y_0, z_0)\]
The tangent plane of \(z = f(x, y)\) at \((x_0, y_0, z_0)\) is
\[- f_x(x - x_0) - f_y(y - y_0) + (z - z_0) = 0\]
\[z = z_0 + f_x(x - x_0) + f_y(y - y_0)\]
\[f(x, y) = f(x_0, y_0) + f_x(x - x_0) + f_y(y - y_0)\]
\end{notn}
\begin{eg}
\(f(x, y) = x^2 + y^2 \quad (x_0, y_0) = (3, 4)\). Approximate \(f(301, 399)\)

\soln
\[\begin{array}{rcl}
f(x, y) & \approx & f(3, 4) + f_x|_{(3, 4)} (x - 3) + f_y|_{(3, 4)} (y - 4)\\
& = & 25 + 6(x - 3) + 8(y - 4)\\
& = & -25  + 6x + 8y
\end{array}\]
\(\implies f(301, 399) \Doteq 25\)
\end{eg}
\section{Chain Rule}
\begin{defn}
\[\displaystyle \frac{d}{dx} (f(g(x)) = \frac{d}{d(g(x))} f(g(x)) \cdot g'(x)\]
\end{defn}
\begin{eg}
\(f(x, y) = x^2 + xy +y^2\) where \(x = \cos t, y = \sin t\). Find \(\displaystyle \frac{d}{dt} f(x(t), y(t))\).

\soln 1
\[\begin{array}{ccl}
f(x(t), y(t)) & = & \cos^2 t + \cos t \sin t + \sin^2 t\\
& = & 1 + \cos t \sin t\\
\displaystyle \frac{d}{dt} f(x(t), y(t)) & = &-\sin^2 t + \cos^2 t
\end{array}\]

\soln 2
\[\begin{array}{rcl}
\displaystyle \frac{d}{dx} f(x(t), y(t)) & = & f_x \cdot x't + f_y \cdot y't\\
& = & (2x + y)(-\sin t) + (x + 2y)(\cos t)\\
& = & (2\cos t + \sin t)(-\sin t) + (\cos t+ 2\sin t)(\cos t)\\
& = & \cos t \sin t(-2 + 2) -\sin^2 t + \cos^2 t\\
& = & -\sin^2 t + \cos^2 t
\end{array}\]
\end{eg}
\begin{notn}
If \(f(x(t, s), y(t, s))\)
\[\begin{array}{rcl}
\displaystyle \frac{\partial f}{\partial t} & = & f_x \cdot x_t + f_y \cdot y_t\\
\displaystyle \frac{\partial f}{\partial s} & = & f_s x_s + f_y y_s
\end{array}\]
\end{notn}
\begin{eg}
\[(x, y) \implies (r, \theta)\]
\[\left\{\begin{array}{rcccl}
x & = & r\cos \theta & = & x(r, \theta)\\
y & = & r\sin \theta & = & y(r, \theta)
\end{array}\right.\]
\end{eg}
\begin{eg}
\(f(x, y) = z = f(x(r, s), y(r, s)), \left\{ \begin{array}{rcccl}
x & = & r^2 + s^2 & = & x(r, s)\\
y & = & 2rs & = & y(r, s)
\end{array}\right.\). Find \(z_{rr}\)

\soln
\[\begin{array}{rcl}
z_r & = & z_x \cdot \cot x_r + z_y \cdot y_r\\
& = & z_x (2r) + z_y(2s)\\
& = & 2(rx_r + sz_y)\\\\
z_{rr} & = & (z_r)_r\\
& = & 2(rz_r + sz_y)_r\\
& = & 2(z_x + 2r^2z_{xx} + 2rs z_{xy} + 2s^2 z_{yy} + 2rs z_{yx})\\\\
(rz_x)_r & = & 1 z_x + r (z_x)_r\\
& = & z_x + r(g_x \cdot x_r + g_y \cdot y_r)\\
& = & z_x + r(z_{xx} (2r) + z_{xy} (2s))\\
& = & z_x + 2r(r z_{xx} + s z_{xy})\\\\
(sz_y)_r & = & s(z_y)_r\\
& = & s(z_{yx} (2r) + z_{yy}(2s))
\end{array}\]
\end{eg}
\begin{eg} 
\(u(x, y) = u(x(r, \theta), y(r, \theta))\). Let \(\left\{\begin{array}{rcl}
x & = & r\cos \theta\\
y & = & r\sin \theta
\end{array}\right.\). Show \(\displaystyle u_{xx} + u_{yy} = u_{rr} + \frac{1}{r} u_r + \frac{1}{r^2} u_{\theta \theta}\)

\soln
\[\begin{array}{rcl}
u_r & = & u_x \cdot x_r + u_y \cdot y_r\\
& = & u_x \cos \theta + u_y \sin \theta\\\\
u_{\theta} & = & u_x \cdot x_{\theta} + u_y \cdot y_{\theta}\\
& = & u_x (-r\sin \theta) + u_y(r\cos \theta)\\\\
u_{rr} & = & (u_r)_r\\
& = & (\cos \theta u_x + \sin \theta u_y)_r\\
& = & \cos \theta (u_x)_r + \sin \theta (u_y)_r\\
& = & \cos \theta ((u_x)_x \cdot x_r + (u_x)_y \cdot y_r) + \sin \theta ((u_y)_x \cdot x_r + (u_y)_y \cdot y_r)\\
& = & u_{xx} (\cos^2 \theta) + u_{yy} (\sin^2 \theta) + u_{xy} (2\cos \theta \sin \theta)\\\\
u_{\theta \theta} & = & (u_\theta)_{\theta}\\
& = & r(-\sin \theta u_x + \cos \theta u_y)_{\theta}\\
& = & r(-\cos \theta u_x -\sin \theta(u_x)_{\theta} - \sin \theta u_y + \cos \theta (u_y)_{\theta}\\
& = & r(-\cos \theta u_x - \sin \theta (u_{xx} \cdot x_{\theta} + u_{xy} \cdot y_{\theta}) - \sin \theta u_y + \cos \theta (u_{yx} \cdot x_{\theta} + u_{yy} \cdot y_{\theta}))\\
& = & u_{xx} (r^2 \sin^2 \theta) +u_{yy} (r^2 \cos^2 \theta) + u_{xy} (2\cos \theta \sin \theta)
\end{array}\]
\[\begin{array}{rcl}
\text{RHS} & = & \displaystyle u_{rr} + \frac{1}{r} u_r + \frac{1}{r^2} u_{\theta \theta}\\
& = & \displaystyle u_{xx} (\cos^2 \theta) + u_{yy} (\sin^2 \theta) + u_{xy} (2\cos \theta \sin \theta) + \frac{\cos \theta}{r} u_x + \frac{\sin \theta}{r} u_y\\
&& \displaystyle + u_{xx} (\sin^2 \theta) + u_{yy} (\cos^2 \theta) + u_{xy} (-2\sin \theta \cos \theta) + \frac{1}{r} (-\cos \theta u_x - \sin \theta u_y)\\
& = & u_{xx} + u_{yy}\\
& = & \text{LHS}
\end{array}\]
\end{eg}